TLB_Page_Tables/MMU_Translate_Refine.thy
@@ -1,6 +1,152 @@
 theory MMU_Translate_Refine
 imports  TLB
+         L3_LIB.L3_Lib
 begin
+
+
+(* page table walk function *)
+
+
+
+definition 
+ConvertAttrsHints'  :: "2 word \<Rightarrow> 4 word"
+where 
+  "ConvertAttrsHints' RGN \<equiv> if RGN = 0x0 then 0x0
+                           else if RGN !! 0 then 
+                                   (if RGN !! 1 then 0xB else 0xF)
+                                else 0xA"
+
+
+definition
+  MemAtt :: "5 word \<Rightarrow> 1 word \<Rightarrow> 32 word \<Rightarrow> 32 word \<Rightarrow> MemoryAttributes"
+where
+  "MemAtt texcb S prrr nmrr \<equiv> if uint ((ucast texcb) :: 3 word) = 6 
+                             then \<lparr>
+                                     MemType         = HOL.undefined  ,
+                                     innerattrs		   = HOL.undefined,
+                                     outerattrs		   = HOL.undefined,
+                                     innerhints		   = HOL.undefined,
+                                     outerhints		   = HOL.undefined,
+                                     innertransient  = False,
+                                     outertransient  = False,
+                                     shareable       = HOL.undefined,
+                                     outershareable  = HOL.undefined \<rparr> 
+                             else (if word_extract (2 * (unat ((ucast texcb) :: 3 word)) + 1) (2 * (unat ((ucast texcb) :: 3 word))) prrr = (0x0 :: 2 word) then 
+                                   \<lparr>
+                                     MemType         = MemType_StronglyOrdered ,
+                                     innerattrs		   = HOL.undefined,
+                                     outerattrs		   = HOL.undefined,
+                                     innerhints		   = HOL.undefined,
+                                     outerhints		   = HOL.undefined,
+                                     innertransient  = False,
+                                     outertransient  = False,
+                                     shareable       = True,
+                                     outershareable  = True \<rparr>  
+                                  else if word_extract (2 * (unat ((ucast texcb) :: 3 word)) + 1) (2 * (unat ((ucast texcb) :: 3 word))) prrr = (0x1 :: 2 word) then 
+                                   \<lparr>
+                                     MemType         = MemType_Device  ,
+                                     innerattrs		   = HOL.undefined,
+                                     outerattrs		   = HOL.undefined,
+                                     innerhints		   = HOL.undefined,
+                                     outerhints		   = HOL.undefined,
+                                     innertransient  = False,
+                                     outertransient  = False,
+                                     shareable       = True,
+                                     outershareable  = True \<rparr>  
+                                  else if word_extract (2 * (unat ((ucast texcb) :: 3 word)) + 1) (2 * (unat ((ucast texcb) :: 3 word))) prrr = (0x2 :: 2 word) then  \<comment> \<open>update this case with the vlaues \<close>
+                                   \<lparr>
+                                     MemType         = MemType_Normal,
+
+                                     innerattrs		   = word_extract 1 0 (ConvertAttrsHints' (word_extract (2 * (unat ((ucast texcb) :: 3 word)) + 1) (2 * (unat ((ucast texcb) :: 3 word))) nmrr)),
+                                     outerattrs		   = word_extract 1 0 (ConvertAttrsHints' (word_extract (2 * (unat ((ucast texcb) :: 3 word)) + 17) (2 * (unat ((ucast texcb) :: 3 word)) +16) nmrr)),
+
+                                     innerhints		   =  word_extract 3 2 (ConvertAttrsHints' (word_extract (2 * (unat ((ucast texcb) :: 3 word)) + 1) (2 * (unat ((ucast texcb) :: 3 word))) nmrr)),
+                                     outerhints		   = word_extract 3 2 (ConvertAttrsHints' (word_extract (2 * (unat ((ucast texcb) :: 3 word)) + 17) (2 * (unat ((ucast texcb) :: 3 word)) +16) nmrr)),
+                                     innertransient  = False,
+                                     outertransient  = False,
+                                     shareable       = if S = 0x0 then prrr!! 18 else prrr !! 19,
+                                     outershareable  = if S = 0x0 then (prrr!! 18) & (\<not>prrr!! ((unat ((ucast texcb) :: 3 word)) + 24)) else (prrr !! 19) & (\<not>prrr!! ((unat ((ucast texcb) :: 3 word)) + 24)) \<rparr>   
+                                    else \<lparr>
+                                     MemType         = HOL.undefined,
+                                     innerattrs		   = HOL.undefined,
+                                     outerattrs		   = HOL.undefined,
+                                     innerhints		   = HOL.undefined,
+                                     outerhints		   = HOL.undefined,
+                                     innertransient  = False,
+                                     outertransient  = False,
+                                     shareable       = HOL.undefined,
+                                     outershareable  = HOL.undefined \<rparr>   ) "
+
+
+
+
+definition
+  perms_to_tlb_fl :: "arm_perm_bits \<Rightarrow> 32 word \<Rightarrow> 32 word \<Rightarrow> flags"
+where
+  "perms_to_tlb_fl pb prrr nmrr \<equiv> \<lparr> 
+   MemoryAttributes = MemAtt (((ucast (arm_p_TEX pb) :: 5 word) << 2) && ((ucast (arm_p_C pb) :: 5 word) << 1) && (ucast (arm_p_B pb) :: 5 word))  (arm_p_S pb) prrr nmrr, 
+   Permissions = \<lparr>ap  = ((ucast (arm_p_APX pb) :: 3 word) << 2)  && ucast(arm_p_AP pb), 
+                         xn = arm_p_XN pb , pxn = arm_p_PXN pb \<rparr>,
+   nG    = arm_p_nG pb,
+   domain  =  arm_p_domain pb,
+   level = arm_p_level pb \<rparr>"
+
+
+type_synonym prrr = "32 word"
+type_synonym nmrr = "32 word"
+
+
+
+definition
+ pt_walk :: "asid \<Rightarrow> heap \<Rightarrow> ttbr0 \<Rightarrow> prrr \<Rightarrow> nmrr \<Rightarrow> vaddr \<Rightarrow> tlb_entry option"
+where
+  "pt_walk  asid heap ttbr0 prrr nmrr v \<equiv>
+      case get_pde heap ttbr0 v
+       of None                 \<Rightarrow> None
+       | Some InvalidPDE       \<Rightarrow> None
+       | Some ReservedPDE      \<Rightarrow> None
+       | Some (SectionPDE p a) \<Rightarrow>
+          Some (EntrySection asid (ucast (addr_val v >> 20) :: 12 word)
+                              (ucast ((addr_val p >> 20) && mask 12) :: 12 word)  (perms_to_tlb_fl a prrr nmrr))
+       | Some (SuperSectionPDE p a) \<Rightarrow>
+         Some (EntrySuper asid   (ucast (addr_val v >> 24) :: 8 word)
+                            (ucast ((addr_val p >> 24) && mask 8) :: 8 word)  (perms_to_tlb_fl a prrr nmrr))
+       | Some (PageTablePDE p) \<Rightarrow>
+               (case get_pte heap p v
+                 of None                     \<Rightarrow> None
+                 |  Some InvalidPTE          \<Rightarrow> None
+                 |  Some (SmallPagePTE p a) \<Rightarrow> 
+                         Some (EntrySmall asid (ucast (addr_val v >> 12) :: 20 word)
+                                             (ucast ((addr_val p >> 12) && mask 20) :: 20 word) (perms_to_tlb_fl a prrr nmrr))
+                 |  Some (LargePagePTE p a) \<Rightarrow> 
+                         Some (EntryLarge asid (ucast (addr_val v >> 16) :: 16 word)
+                                             (ucast ((addr_val p >> 16) && mask 16) :: 16 word) (perms_to_tlb_fl a prrr nmrr)))"
+
+
+
+
+record AdrDes = phy_ad :: paddr
+                memattrs :: MemoryAttributes 
+
+
+
+definition
+  ptable_lift_adrdesc :: "heap \<Rightarrow> paddr  \<Rightarrow> prrr \<Rightarrow> prrr \<Rightarrow> vaddr \<rightharpoonup> AdrDes" where
+  "ptable_lift_adrdesc h pt_root prrr nmrr vp \<equiv>
+     let
+       vp_val = addr_val vp
+     in
+       map_option 
+         (\<lambda>(base, pg_size, perms). 
+            \<lparr>phy_ad = base r+ (vaddr_offset pg_size vp_val),
+             memattrs = MemAtt (((ucast (arm_p_TEX perms) :: 5 word) << 2) && ((ucast (arm_p_C perms) :: 5 word) << 1) && (ucast (arm_p_B perms) :: 5 word))  (arm_p_S perms) prrr nmrr \<rparr>)
+         (lookup_pde h pt_root vp)"
+
+
+
+(* building up new state *)
+
+
 
 
 datatype Exception =
@@ -13,20 +159,21 @@ datatype Exception =
 
 
 record cstate =
-  mem :: "paddr \<rightharpoonup> byte"
+  heap :: "paddr \<rightharpoonup> byte"
   ttbr0 :: paddr 
   asid :: asid
   Exception :: Exception
-  data_exe :: bool
   prrr :: "32 word" \<comment> \<open>for memory attributes\<close>
   nmrr :: "32 word" \<comment> \<open>for memory attributes\<close>
+  dacr :: "32 word" \<comment> \<open>for domain\<close>
 
 
 
+(*
 definition 
-  raise'exception  :: "Exception \<Rightarrow> 'a cstate_scheme \<Rightarrow> 'r \<times> 'a cstate_scheme"
+  raise'exception'  :: "Exception \<Rightarrow> 'a cstate_scheme \<Rightarrow> 'r \<times> 'a cstate_scheme"
 where 
-  "raise'exception \<equiv> \<lambda>e. do {
+  "raise'exception' \<equiv> \<lambda>e. do {
                         v \<leftarrow> read_state Exception;
                         _ \<leftarrow> do {
                             b \<leftarrow> return (v = NoException);
@@ -34,11 +181,19 @@ where
                           };
                         return HOL.undefined
                       }"
+*)
+
+definition 
+  raise'exception'  :: "Exception \<Rightarrow> 'a cstate_scheme \<Rightarrow> 'r \<times> 'a cstate_scheme"
+where 
+  "raise'exception' \<equiv> \<lambda>e s. let (v, s) = (Exception s, s); (u, y) = let (b, y) = (v = NoException, s) in (if b then \<lambda>s. ((), s\<lparr>Exception := e\<rparr>) else Pair ()) y in (undefined, y)"
 
 
 
+(* classes proto-types *)
+(* should we take vaddr in the end of the inputs?*)
 class mmu =
-  fixes mmu_translate :: "vaddr \<Rightarrow> 'a cstate_scheme \<Rightarrow> (paddr \<times> MemoryAttributes) \<times> 'a cstate_scheme" 
+  fixes mmu_translate :: "vaddr \<Rightarrow> nat \<Rightarrow> bool \<Rightarrow> bool \<Rightarrow> bool \<Rightarrow>'a cstate_scheme \<Rightarrow> (paddr \<times> MemoryAttributes) \<times> 'a cstate_scheme" 
 
 class mem_op = mmu +
   fixes mmu_read :: "vaddr \<Rightarrow> 'a cstate_scheme \<Rightarrow> bool list \<times> 'a cstate_scheme"
@@ -79,7 +234,7 @@ lemma tlbs_truncate [simp]:
   by (clarsimp simp: typ_tlbs_def cstate.defs)
 
 lemma typ_tlbs_prim_parameter [simp]:
-  "asid (typ_tlbs s) = asid s \<and> ttbr0 (typ_tlbs s) =  ttbr0 s \<and> mem (typ_tlbs s) = mem s \<and>
+  "asid (typ_tlbs s) = asid s \<and> ttbr0 (typ_tlbs s) =  ttbr0 s \<and> heap (typ_tlbs s) = heap s \<and>
       Exception (typ_tlbs s) = Exception s"
   by (clarsimp simp: typ_tlbs_def  cstate.defs)
 
@@ -93,14 +248,6 @@ consts unitlb_evict :: "tlbs_set cstate_scheme \<Rightarrow> tlb_entry set"
 
 *)
 
-fun
-  flags_entry :: "tlb_entry \<Rightarrow> flags"
-where
-  "flags_entry (EntrySmall   a x y fl) = fl"
-| "flags_entry (EntryLarge   a x y fl) = fl"
-| "flags_entry (EntrySection a x y fl) = fl"
-| "flags_entry (EntrySuper   a x y fl) = fl"
-
 
 definition 
   tlb_entry_to_adrdesc :: "vaddr \<Rightarrow> tlb_entry \<Rightarrow> (paddr \<times> MemoryAttributes)"
@@ -108,14 +255,70 @@ where
   "tlb_entry_to_adrdesc v entry = ((Addr (va_to_pa (addr_val v) entry)),
                                        MemoryAttributes(flags_entry entry))"
 
-(* address check and return the address descriptor  *)
 
-(* we should remove evict from here  *)
+definition 
+  MemType_entry :: "tlb_entry \<Rightarrow> MemType_t" 
+where
+  "MemType_entry e = MemType (MemoryAttributes (flags_entry e))"
+
+definition 
+Align' :: "'a::len0 word \<times> nat \<Rightarrow> 'a word"
+where
+  "Align' \<equiv> \<lambda>(w, n). word_of_int (int (n * (nat (uint w) div n)))"
+
+
+
+
+definition 
+CheckDomain' :: "4 word \<Rightarrow> 32 word  \<Rightarrow> 32 word \<Rightarrow> bool option"
+where
+  "CheckDomain' dm va dcr \<equiv> 
+           if word_extract (2 * (unat dm) + 1) (2 * (unat dm)) dcr = (0x0 :: 2 word) then None
+           else if  word_extract (2 * (unat dm) + 1) (2 * (unat dm)) dcr = (0x1 :: 2 word) then Some True
+           else if  word_extract (2 * (unat dm) + 1) (2 * (unat dm)) dcr = (0x2 :: 2 word) then None
+           else Some False"
+
+
+definition 
+CheckPermission' :: "Permissions \<Rightarrow> bool  \<Rightarrow> bool \<Rightarrow> bool option"
+where
+  "CheckPermission' perm ispriv iswrite \<equiv> 
+             if ap (perm) = 0x0 then  Some True
+             else if ap (perm) = 0x1 then  Some (\<not>ispriv)
+             else if ap (perm) = 0x2 then  Some (\<not>ispriv & iswrite)
+             else if ap (perm) = 0x3 then  Some False
+             else if ap (perm) = 0x4 then  None
+             else if ap (perm) = 0x5 then  Some (\<not>ispriv \<or> iswrite)
+             else if ap (perm) = 0x6 then  Some iswrite
+             else Some iswrite"
+
+
+
+
+
+definition 
+  align_dom_perm_entry_check  :: "tlb_entry \<Rightarrow> vaddr \<Rightarrow> nat \<Rightarrow> 32 word \<Rightarrow> bool \<Rightarrow> bool \<Rightarrow> 'a cstate_scheme \<Rightarrow> (paddr \<times> MemoryAttributes) \<times> 'a cstate_scheme" 
+where 
+  "align_dom_perm_entry_check \<equiv> \<lambda> entry v siz dacr ispriv iswrite. if (MemType_entry entry = MemType_Device \<or> MemType_entry entry = MemType_StronglyOrdered) \<and> addr_val v \<noteq> Align' (addr_val v, siz)  
+                                         then raise'exception' (MMU_Exception ''Alignment Fault'')
+                                         else do {
+                                                  let chkdm = CheckDomain' (domain (flags_entry entry)) (addr_val v) dacr;
+                                                  if chkdm = None then raise'exception' (MMU_Exception ''Domain Fault'')  else
+                                                  if chkdm = Some True then  
+                                                          do{let chkprm = CheckPermission' (Permissions (flags_entry entry)) ispriv iswrite;  \<comment> \<open>encodes abort\<close>
+                                                               if chkprm = None then raise'exception' (MMU_Exception ''Permission Fault'')
+                                                                else if  chkprm = Some True then raise'exception' (MMU_Exception ''Permission Fault'')
+                                                                else return (tlb_entry_to_adrdesc v entry)}
+                                                    else return (tlb_entry_to_adrdesc v entry)}"
+
+
+
+
 
 instantiation tlb_state_ext :: (type) mmu   
 begin
   definition   
-  "(mmu_translate v :: ('a tlb_state_scheme \<Rightarrow> _))
+  "(mmu_translate v siz ispriv iswrite data_ins :: ('a tlb_state_scheme \<Rightarrow> _))
   = do {
      \<comment> \<open>tlbs  <- read_state tlbs_set;
      update_state (\<lambda>s. s\<lparr> tlbs_set :=  tlbs \<lparr> dtlb_set   := dtlb_set tlbs  -  dtlb_evict(typ_tlbs s) ,
@@ -125,49 +328,47 @@ begin
      let dtlb =  dtlb_set tlbs;
      let itlb =  itlb_set tlbs;
      let maintlb =  unitlb_set tlbs;
-     df    <- read_state data_exe;
-     mem   <- read_state mem;
+     heap   <- read_state heap;
      asid  <- read_state asid;
      ttbr0 <- read_state ttbr0;
      prrr  <- read_state prrr;
      nmrr  <- read_state nmrr;
-     if df then
+     dacr <- read_state dacr;
+     if data_ins then
            case lookup dtlb asid (addr_val v) of
-                Hit entry \<Rightarrow>  return (tlb_entry_to_adrdesc v entry)
+                Hit entry \<Rightarrow>  align_dom_perm_entry_check entry v siz dacr ispriv iswrite
               | Miss \<Rightarrow> (case lookup maintlb asid (addr_val v) of
-                             Hit entry \<Rightarrow>  return (tlb_entry_to_adrdesc v entry)
-                          |  Miss \<Rightarrow> (case pt_walk asid mem ttbr0 prrr nmrr v of 
-                                            None \<Rightarrow> raise'exception (MMU_Exception ''more info'')
+                             Hit entry \<Rightarrow> align_dom_perm_entry_check entry v siz dacr ispriv iswrite
+                          |  Miss \<Rightarrow> (case pt_walk asid heap ttbr0 prrr nmrr v of 
+                                            None \<Rightarrow> raise'exception' (MMU_Exception ''more info'')
                                          |  Some entry \<Rightarrow> do {
+                                                 \<comment> \<open>it seems like from the manual that TLB is loaded first, alignment and  domain checking is performed afterwards\<close>
                                                  let tlb_rld = tlbs \<lparr> dtlb_set := dtlb \<union> {entry}, 
                                                                        unitlb_set := maintlb \<union> {entry} \<rparr>;
                                                  update_state (\<lambda>s. s\<lparr> tlbs_set := tlb_rld \<rparr>);
-                                                 return (tlb_entry_to_adrdesc v entry)
-                                             } )
-                          | Incon \<Rightarrow> raise'exception (IMPLEMENTATION_DEFINED ''set on fire''))
-              | Incon \<Rightarrow> raise'exception (IMPLEMENTATION_DEFINED ''set on fire'') 
+                                                 align_dom_perm_entry_check entry v siz dacr ispriv iswrite })
+                          | Incon \<Rightarrow> raise'exception' (IMPLEMENTATION_DEFINED ''set on fire''))
+              | Incon \<Rightarrow> raise'exception' (IMPLEMENTATION_DEFINED ''set on fire'') 
           else 
            case lookup itlb asid (addr_val v) of
-                Hit entry \<Rightarrow>  return (tlb_entry_to_adrdesc v entry)
+                Hit entry \<Rightarrow>  align_dom_perm_entry_check entry v siz dacr ispriv iswrite
               | Miss \<Rightarrow> (case lookup maintlb asid (addr_val v) of
-                             Hit entry \<Rightarrow>  return (tlb_entry_to_adrdesc v entry)
-                          |  Miss \<Rightarrow> (case pt_walk asid mem ttbr0 prrr nmrr v of 
-                                            None \<Rightarrow> raise'exception (MMU_Exception ''more info'')
-                                         |  Some entry \<Rightarrow> do {
+                             Hit entry \<Rightarrow>  align_dom_perm_entry_check entry v siz dacr ispriv iswrite
+                          |  Miss \<Rightarrow> (case pt_walk asid heap ttbr0 prrr nmrr v of 
+                                            None \<Rightarrow> raise'exception' (MMU_Exception ''more info'')
+                                        |  Some entry \<Rightarrow> do {
+                                                 \<comment> \<open>it seems like from the manual that TLB is loaded first, alignment and  domain checking is performed afterwards\<close>
                                                  let tlb_rld = tlbs \<lparr> itlb_set := itlb \<union> {entry}, 
                                                                        unitlb_set := maintlb \<union> {entry} \<rparr>;
                                                  update_state (\<lambda>s. s\<lparr> tlbs_set := tlb_rld \<rparr>);
-                                                 return (tlb_entry_to_adrdesc v entry)
-                                             } )
-                          | Incon \<Rightarrow> raise'exception (IMPLEMENTATION_DEFINED ''set on fire''))
-              | Incon \<Rightarrow> raise'exception (IMPLEMENTATION_DEFINED ''set on fire'') 
+                                                 align_dom_perm_entry_check entry v siz dacr ispriv iswrite })
+                          | Incon \<Rightarrow> raise'exception' (IMPLEMENTATION_DEFINED ''set on fire''))
+              | Incon \<Rightarrow> raise'exception' (IMPLEMENTATION_DEFINED ''set on fire'') 
    }"
 
-thm mmu_translate_tlb_state_ext_def
-(* print_context *)                      
+thm mmu_translate_tlb_state_ext_def                     
   instance ..
 end
-
 
 
 end
